examples/formal-languages/context-free/pegSampleScript.sml
@@ -70,15 +70,15 @@ end
 val result1 = save_thm(
   "result1",
   time EVAL ``peg_exec ^G (nt (INL "expr") I)
-                      [Number 1; Plus; Number 2; Times; Number 4] []
+                      (map_loc [Number 1; Plus; Number 2; Times; Number 4] 0) []
                       done failed``)
 
 (* As of 5a18cdc17ff, takes 1.983s (ugh) *)
 val result2 = save_thm(
   "result2",
   time EVAL ``peg_exec ^G (nt (INL "expr") I)
-                      [Number 1; Plus; Number 2; Times; Number 4;
-                       Times; LParen; Number 3; Plus; Number 1; RParen]
+                      (map_loc [Number 1; Plus; Number 2; Times; Number 4;
+                       Times; LParen; Number 3; Plus; Number 1; RParen] 0)
                       [] done failed``)
 
 val G_def = zDefine`G = <| start := nt (INL "expr") I; rules := ^rules |>`
@@ -103,8 +103,8 @@ val _ = computeLib.add_persistent_funs ["Grules"]
 val result2' = save_thm(
   "result2'",
   time EVAL ``peg_exec G (nt (INL "expr") I)
-                      [Number 1; Plus; Number 2; Times; Number 4;
-                       Times; LParen; Number 3; Plus; Number 1; RParen]
+                      (map_loc [Number 1; Plus; Number 2; Times; Number 4;
+                       Times; LParen; Number 3; Plus; Number 1; RParen] 0)
                       [] done failed``)
 
 
